Test/civl/regression-tests/intro-nonblocking.bpl
@@ -1,7 +1,0 @@
-// RUN: %parallel-boogie "%s" > "%t"
-// RUN: %diff "%s.expect" "%t"
-
-pure action intro (x:int)
-{
-  assume x == 0;
-}
