Test/civl/paxos/is.sh
@@ -3,4 +3,4 @@
 # RUN: %parallel-boogie Paxos.bpl PaxosActions.bpl PaxosImpl.bpl /lib:set_size /timeLimit:120 > "%t"
 # RUN: %diff "%s.expect" "%t"
 
-boogie $@ Paxos.bpl PaxosActions.bpl PaxosImpl.bpl
+boogie $@ /lib:set_size Paxos.bpl PaxosActions.bpl PaxosImpl.bpl
